## Enunciado
Con las matrices del ejercicio 1, realizar
 - a)
 - b)

## Ayuda
$M = A$ (simetrica) + $B$ (antisimetrica)

$$A = \frac{M+M^t}{2} = \frac{1}{2} (M+M^t)$$

$$B = \frac{M - M^t}{2} = \frac{1}{2} (M-M^t)$$

## a)
$$
M=\begin{pmatrix}
3 & 2 & -1 \\
4 & 5 & 0
\end{pmatrix} \begin{pmatrix}
1 & -1 \\
0 & 2 \\
5 & 2
\end{pmatrix} = \begin{pmatrix}
-2 & -1 \\
4 & 6
\end{pmatrix}
$$
$$
L = \begin{pmatrix}
3 & 4 \\
2 & 5 \\
-1 & 0
\end{pmatrix}\begin{pmatrix}
-1 & 0 & 2 \\
4 & 3 & -2
\end{pmatrix} = \begin{pmatrix}
13 & 12 & -2 \\
18 & 15 & -6 \\
1 & 0 & -2
\end{pmatrix}
$$